More stuff in bucketsort implementation.

boogie/bucketsort.bpl
@@ -31,13 +31,41 @@ procedure BucketSort (input: Array, count: int) returns (result, permutation: Ar
   ensures is_permutation (permutation, count);
   ensures (forall i:int :: 0 <= i && i < count ==> result [i] == input [permutation[i]]);
 {
-  var tmp: int;
+  var tmp, value: int;
+  var left, middle, right: Array;
+  var left_count, middle_count, right_count: int;
+  
   tmp := 0;
+  left_count := 0;
+  middle_count := 0;
+  right_count := 0;
+  
+  
   while (tmp <= count)
     invariant (forall i:int :: 0 <= i && i < tmp ==> permutation [i] == i && input [i] == result [i]);
+    invariant (forall i: int :: 0 <= i && i < left_count ==> -3*N <= left [i] && left [i] < -N);
+    invariant (forall i: int :: 0 <= i && i < middle_count ==> -N <= middle [i] && middle [i] <= N);
+    invariant (forall i: int :: 0 <= i && i < right_count ==> N < right [i] && right [i] <= 3*N);
   {
+    value := input [tmp];
+    if (value < -N) {
+      left [left_count] := value;
+      left_count := left_count + 1;
+    } else {
+      if (value <= N) {
+        middle [middle_count] := value;
+        middle_count := middle_count + 1;
+      } else {
+        right [right_count] := value;
+        right_count := right_count + 1;
+      }
+    }
+    
     permutation [tmp] := tmp;
     result [tmp] := input [tmp];
     tmp := tmp + 1;
   }
+  
+  
+  
 }
